pico-ifc-coq/basic_machines/CLattices.v
@@ -111,6 +111,7 @@ Proof.
   intuition; eauto.
 Qed.
 
+
 Lemma genFlows_spec_HL: forall Q,
    HT  genFlows
        (fun m s => exists l l' s0, s = (labToZ l, handlerTag) :::
